LogRel/STLC/SN.lean
@@ -8,14 +8,21 @@ def halts (e : Expr) :=
 
 @[simp]
 def SN : Expr → Ty → Prop
-  | e, .unit => lc e ∧ halts e
-  | f, .arrow τ𝕒 τ𝕓 => lc f ∧ halts f ∧ ∀ arg, SN arg τ𝕒 → SN (.app f arg) τ𝕓
+  | e, .unit => closed e ∧ lc e ∧ halts e
+  | f, .arrow τ𝕒 τ𝕓 => closed f ∧ lc f ∧ halts f ∧ ∀ arg, SN arg τ𝕒 → SN (.app f arg) τ𝕓
 
 theorem SN_impl_halts : ∀ e τ, SN e τ → halts e := by
   intros e τ HSN
   induction τ
-  case unit => apply HSN.right
-  case arrow => apply HSN.right.left
+  case unit => apply HSN.right.right
+  case arrow => apply HSN.right.right.left
+
+theorem closed_step : ∀ e₀ e₁, step e₀ e₁ → (closed e₀ ↔ closed e₁) :=
+  by
+  intros e₀ e₁ Hstep
+  constructor
+  . admit
+  . admit
 
 theorem lc_step : ∀ e₀ e₁, step e₀ e₁ → (lc e₀ ↔ lc e₁) :=
   by
@@ -41,41 +48,57 @@ theorem SN_step : ∀ e₀ e₁ τ, step e₀ e₁ → (SN e₀ τ ↔ SN e₁ �
   . intros HSN₀
     induction τ generalizing e₀ e₁
     case unit =>
+      have ⟨Hclosed, Hlc, Hhalts⟩ := HSN₀
+      constructor
+      . apply (closed_step _ _ _).mp
+        apply Hclosed; apply Hstep
       constructor
       . apply (lc_step _ _ _).mp
-        apply HSN₀.left; apply Hstep
+        apply Hlc; apply Hstep
       . apply (halts_step _ _ _).mp
-        apply HSN₀.right; apply Hstep
+        apply Hhalts; apply Hstep
     case arrow IHa IHb =>
+      have ⟨Hclosed, Hlc, Hhalts, IH⟩ := HSN₀
+      constructor
+      . apply (closed_step _ _ _).mp
+        apply Hclosed; apply Hstep
       constructor
       . apply (lc_step _ _ _).mp
-        apply HSN₀.left; apply Hstep
-      . constructor
-        . apply (halts_step _ _ _).mp
-          apply HSN₀.right.left; apply Hstep
-        . intro arg HSN₁
-          apply IHb
-          apply step_appl; apply Hstep
-          apply HSN₀.right.right; apply HSN₁
+        apply Hlc; apply Hstep
+      constructor
+      . apply (halts_step _ _ _).mp
+        apply Hhalts; apply Hstep
+      . intro arg HSN₁
+        apply IHb
+        apply step_appl; apply Hstep
+        apply IH; apply HSN₁
   . intros HSN₀
     induction τ generalizing e₀ e₁
     case unit =>
+      have ⟨Hclosed, Hlc, Hhalts⟩ := HSN₀
+      constructor
+      . apply (closed_step _ _ _).mpr
+        apply Hclosed; apply Hstep
       constructor
       . apply (lc_step _ _ _).mpr
-        apply HSN₀.left; apply Hstep
+        apply Hlc; apply Hstep
       . apply (halts_step _ _ _).mpr
-        apply HSN₀.right; apply Hstep
+        apply Hhalts; apply Hstep
     case arrow IHa IHb =>
+      have ⟨Hclosed, Hlc, Hhalts, IH⟩ := HSN₀
+      constructor
+      . apply (closed_step _ _ _).mpr
+        apply Hclosed; apply Hstep
       constructor
       . apply (lc_step _ _ _).mpr
-        apply HSN₀.left; apply Hstep
-      . constructor
-        . apply (halts_step _ _ _).mpr
-          apply HSN₀.right.left; apply Hstep
-        . intro arg HSN₁
-          apply IHb
-          apply step_appl; apply Hstep
-          apply HSN₀.right.right; apply HSN₁
+        apply Hlc; apply Hstep
+      constructor
+      . apply (halts_step _ _ _).mpr
+        apply Hhalts; apply Hstep
+      . intro arg HSN₁
+        apply IHb
+        apply step_appl; apply Hstep
+        apply IH; apply HSN₁
 
 theorem SN_stepn : ∀ e₀ e₁ τ, stepn e₀ e₁ → (SN e₀ τ ↔ SN e₁ τ) :=
   by
@@ -115,10 +138,14 @@ theorem fundamental : ∀ Γ e τ γs, typing Γ e τ → SN_Env γs Γ → SN (
   case lam e _ _ _ HFv IH =>
     constructor
     . admit
-    . constructor; exists substs γs (.lam e)
-      constructor; constructor
-      apply stepn.refl
-      intro arg HSN
+    constructor
+    . admit
+    constructor
+    . exists substs γs (.lam e)
+      constructor
+      . constructor
+      . apply stepn.refl
+    . intro arg HSN
       have ⟨v, Hvalue, Hstepn⟩ := SN_impl_halts _ _ HSN
       apply (SN_stepn _ _ _ _).mpr; apply IH (v :: γs); apply SN_Env.cons
       apply (SN_stepn _ _ _ _).mp; apply HSN; apply Hstepn; apply HSNΓ
@@ -127,9 +154,11 @@ theorem fundamental : ∀ Γ e τ γs, typing Γ e τ → SN_Env γs Γ → SN (
       rw [← SN_Env_impl_length_eq _ _ HSNΓ, ← subst_intro γs.length, ← substs_opening_comm]
       all_goals admit
   case app IH₀ IH₁ =>
-    apply (IH₀ _ HSNΓ).right.right
+    apply (IH₀ _ HSNΓ).right.right.right
     apply IH₁ _ HSNΓ
   case unit =>
+    constructor
+    . simp
     constructor
     . constructor
     . exists .unit
